\documentclass[11pt, a4paper]{article}
%\usepackage{proj1}
\usepackage{natbib}
\usepackage{fancyhdr}  
\usepackage{subcaption}
\usepackage{caption}
\usepackage{graphicx}
\linespread{1.25} 
\setlength{\parindent}{0cm}
\graphicspath{{Images/}}
\usepackage{hyperref}
\usepackage{amsmath}
\usepackage{amsfonts}
\usepackage{amssymb}
\usepackage{amsthm}
\usepackage{mathtools}
\usepackage{commath}

%\usepackage[sc,osf]{mathpazo}
\usepackage{subcaption}
\usepackage[a4paper, top=1in, left=1.0in, right=1.0in, bottom=1in, includehead, includefoot]{geometry} %Usually have top as 1in

\usepackage{listings}
\usepackage{color} %red, green, blue, yellow, cyan, magenta, black, white
\definecolor{mygreen}{RGB}{28,172,0} % color values Red, Green, Blue
\definecolor{mylilas}{RGB}{170,55,241}


\hypersetup{colorlinks,linkcolor={black},citecolor={blue},urlcolor={black}}
\usepackage{color}
\urlstyle{same}


\theoremstyle{definition}
\newtheorem{definition}{Definition}[section]

\title{Exact Solutions for the Full Problem \\with Force Control and with Flow Control}
\date{}
\newcommand{\Sta}{\rho}
\newcommand{\Adj}{p}
\newcommand{\Con}{u}

\pagenumbering{gobble}
\begin{document}
\lstset{language=Matlab,%
	%basicstyle=\color{red},
	breaklines=true,%
	morekeywords={matlab2tikz},
	keywordstyle=\color{blue},%
	morekeywords=[2]{1}, keywordstyle=[2]{\color{black}},
	identifierstyle=\color{black},%
	stringstyle=\color{mylilas},
	commentstyle=\color{mygreen},%
	showstringspaces=false,%without this there will be a symbol in the places where there is a space
	numbers=left,%
	numberstyle={\tiny \color{black}},% size of the numbers
	numbersep=9pt, % this defines how far the numbers are from the text
	emph=[1]{for,end,break},emphstyle=[1]\color{blue}, %some words to emphasise
	%emph=[2]{word1,word2}, emphstyle=[2]{style},    
    basicstyle=\footnotesize\ttfamily,
}
	
\maketitle

\section*{The Equations: Force Control}
\textbf{Forward Problem}
\begin{align*}
&\partial_t \Sta = \nabla^2 \Sta - \nabla \cdot (\rho \mathbf{w}_{Flow}) + \nabla \cdot (\Sta \nabla V_{ext}) +{w}_{Force} + f \\
& \Sta = \Sta_0 \quad \text{at} \quad t=0.  \notag
\end{align*}
\begin{align*}
&\text{No-Flux}\\
&\dfrac{\partial \Sta}{\partial n} - \Sta \mathbf{w}_{Flow} \cdot \mathbf{n} + \Sta \dfrac{\partial V_{ext}}{\partial n}  =0  \\
&\text{Dirichlet}\\
&\Sta =0 
\end{align*}
\textbf{Adjoint Equation}
\begin{align*}
\partial_t \Adj &= -\Sta + \hat \Sta -  \nabla \Adj \cdot \mathbf w_{Flow} -  \nabla^2 \Adj +  \nabla \Adj \cdot \nabla V_{ext} \\
\Adj(r,T)&=0
\end{align*}
\begin{align*}
\text{No-Flux}  \notag\\
\frac{\partial \Adj }{\partial n}&=0,  \notag\\
\text{Dirichlet}\\
\Adj&=0.
\end{align*}




\textbf{Gradient Equation}
\begin{align*}
{w}_{Force}=-\frac{1}{\beta}\Adj
\end{align*} 



\section*{Exact Solutions: Force Control}
(+++ Just a very small adaptation from John's notes!+++)

\subsection*{Dirichlet BCs}
We choose:
\begin{align*}
\Sta &= 2 e^t \cos(\frac{\pi x}{2})\\
\Adj &=(e^T-e^t) \cos(\frac{\pi x}{2})\\
V_{ext} &= \frac{1}{2} \cos(\frac{\pi x}{2})
\end{align*}
The expression for $V_{ext}$ is chosen such that $V_{ext}= \frac{1}{2}V_{extOld}  $, where $V_{extOld}=\cos(\frac{\pi x}{2})$ is taken from John's notes. Then a valid choice of $\mathbf{w}_{Flow}$ is  $\frac{1}{2} \nabla V_{extOld}$:
\begin{align*}
\mathbf{w}_{Flow}= -\frac{1}{2} \nabla \cos(\frac{\pi x}{2}) = \frac{\pi}{4} \sin(\frac{\pi x}{2}).
\end{align*}
Note that it can be verified that $ \mathbf{w}_{Flow} - \nabla V_{ext}= - \nabla V_{extOld}$.
Therefore, the expressions for $w_{Force}$, $f$ and $\hat \Sta$ are the same as in John's notes:
\begin{align*}
w_{Force}= -\frac{1}{\beta}(e^T - e^t)\cos(\frac{\pi x}{2}),
\end{align*}
which follows from the gradient equation and the choice of $\Adj$.
Also, from computations and choice of $\Sta$,$\Adj$ and $V_{ext}$, we get:
\begin{align*}
f&= \bigg( (2  + \frac{\pi^2}{2} -\frac{1}{\beta} )e^t  + \frac{1}{\beta}e^T  \bigg)\cos(\frac{\pi x}{2}) - \frac{\pi^2}{2}e^t \bigg( \sin^2(\frac{\pi x}{2}) - \cos^2(\frac{\pi x}{2})\bigg)\\
\hat \Sta &= e^t \cos(\frac{\pi x}{2})- \frac{\pi^2}{4}(e^T -e^t)\cos(\frac{\pi x}{2}) - \frac{\pi^2}{4}(e^T -e^t)\sin^2(\frac{\pi x}{2})
\end{align*}




\subsection*{Neumann BCs}

We choose:
\begin{align*}
\Sta &= 2 e^t \cos(\pi x)\\
\Adj &=(e^T-e^t) \cos(\pi x)\\
V_{ext} &= \frac{1}{2} \cos(\pi x)
\end{align*}
The expression for $V_{ext}$ is again chosen such that $V_{ext}= \frac{1}{2}V_{extOld}  $, where $V_{extOld}=\cos(\pi x)$ is taken from John's notes. Then a valid choice of $\mathbf{w}_{Flow}$ is  $\frac{1}{2} \nabla V_{extOld}$:
\begin{align*}
\mathbf{w}_{Flow}= -\frac{1}{2} \nabla \cos(\pi x) = \frac{\pi}{2} \sin(\pi x).
\end{align*}
Note that it can be verified that $ \mathbf{w}_{Flow} - \nabla V_{ext}= - \nabla V_{extOld}$.
Therefore, the expressions for $w_{Force}$, $f$ and $\hat \Sta$ are again the same as in John's notes:
\begin{align*}
w_{Force}= -\frac{1}{\beta}(e^T - e^t)\cos(\pi x),
\end{align*}
which follows from the gradient equation and the choice of $\Adj$.
Also, from computations and choice of $\Sta$,$\Adj$ and $V_{ext}$, we get:
\begin{align*}
f&= \bigg( (2  + 2\pi^2 -\frac{1}{\beta} )e^t  + \frac{1}{\beta}e^T  \bigg)\cos(\pi x) - 2\pi^2e^t \bigg( \sin^2(\pi x) - \cos^2(\pi x)\bigg)\\
\hat \Sta &= e^t \cos(\pi x)- \pi^2(e^T -e^t)\cos(\pi x) - \pi^2(e^T -e^t)\sin^2(\pi x)
\end{align*}


\section*{The Equations: Flow Control}
\textbf{Forward Problem}
\begin{align*}
&\partial_t \Sta = \nabla^2 \Sta - \nabla \cdot (\rho \mathbf{w}_{Flow}) + \nabla \cdot (\Sta \nabla V_{ext}) +{w}_{Force} + f \\
& \Sta = \Sta_0 \quad \text{at} \quad t=0.  \notag
\end{align*}
\begin{align*}
&\text{No-Flux}\\
&\dfrac{\partial \Sta}{\partial n} - \Sta \mathbf{w}_{Flow} \cdot \mathbf{n} + \Sta \dfrac{\partial V_{ext}}{\partial n}  =0  \\
&\text{Dirichlet}\\
&\Sta =0 
\end{align*}
\textbf{Adjoint Equation}
\begin{align*}
\partial_t \Adj &= -\Sta + \hat \Sta -  \nabla \Adj \cdot \mathbf w_{Flow} -  \nabla^2 \Adj +  \nabla \Adj \cdot \nabla V_{ext} \\
\Adj(r,T)&=0
\end{align*}
\begin{align*}
\text{No-Flux}  \notag\\
\frac{\partial \Adj }{\partial n}&=0,  \notag\\
\text{Dirichlet}\\
\Adj&=0.
\end{align*}
\textbf{Gradient Equation                             }
\begin{align*}
\mathbf w_{Flow}=-\frac{1}{\beta}\Sta \nabla \Adj
\end{align*} 





\section*{Exact Solutions: Flow Control}
(+++ Just a very small adaptation from John's notes!+++)

\subsection*{Dirichlet BCs}
We choose:
\begin{align*}
\Sta &= 2 e^t \cos(\frac{\pi x}{2})\\
\Adj &=(e^T-e^t) \cos(\frac{\pi x}{2})
\end{align*}
Then, from the gradient equation we find that:
\begin{align*}
\mathbf{w}_{Flow }= \frac{\pi}{\beta}e^t(e^T -e^t)\cos(\frac{\pi x}{2}) \sin(\frac{\pi x}{2}).
\end{align*}
Then we need to solve the forward equation using these quantities. That is:
\begin{align*}
\partial_t \Sta - \nabla^2 \Sta + \nabla \cdot (\rho \mathbf{w}_{Flow}) = \nabla \cdot (\Sta \nabla V_{ext}) +{w}_{Force} + f.
\end{align*}
One choice is to set:
\begin{align*}
\nabla \cdot (\rho \mathbf{w}_{Flow}) = \nabla \cdot (\Sta \nabla V_{ext}),
\end{align*}
which implies that
\begin{align*}
 \mathbf{w}_{Flow} &= \nabla V_{ext} \\
 &=\frac{\pi}{\beta}e^t(e^T -e^t)\cos(\frac{\pi x}{2}) \sin(\frac{\pi x}{2}).
\end{align*}
Then, integrating this, we find $V_{ext}$:
\begin{align*}
V_{ext} &= \int_\Omega \frac{\pi}{\beta}e^t(e^T -e^t)\cos(\frac{\pi x}{2}) \sin(\frac{\pi x}{2}) dx\\
&=\frac{1}{\beta}e^t(e^T -e^t)\sin^2(\frac{\pi x}{2}).
\end{align*}
Since we know that $\nabla \cdot (\rho \mathbf{w}_{Flow}) = \nabla \cdot (\Sta \nabla V_{ext})$, the remaining terms to balance are:
\begin{align*}
\partial_t \Sta - \nabla^2 \Sta  = {w}_{Force} + f.
\end{align*}
Then
\begin{align*}
 {w}_{Force} + f = (2 + \frac{\pi^2}{2}) e^t \cos(\frac{\pi x}{2}), 
\end{align*}
where ${w}_{Force} + f$ is one force term.
Now $\hat \Sta $ can be found using the adjoint equation:
\begin{align*}
\partial_t \Adj &=- \Sta + \hat \Sta -  \nabla \Adj \cdot \mathbf w_{Flow} -  \nabla^2 \Adj +  \nabla \Adj \cdot \nabla V_{ext},
\end{align*}
which reduces to:
\begin{align*}
\partial_t \Adj &= \Sta - \hat \Sta  -  \nabla^2 \Adj,
\end{align*}
due to the choices of $\mathbf{w}_{Flow}$ and $V_{ext}$, which gives:
\begin{align*}
 \hat \Sta &= \partial_t \Adj +\Sta   +  \nabla^2 \Adj\\
 &=(1-\frac{\pi^2}{4})e^t\cos(\frac{\pi x}{2}) +\frac{\pi^2}{4}e^t \cos(\frac{\pi x}{2}).
\end{align*}












\subsection*{Neumann BCs}
Choose scaling factors $c \beta $ in $\mathbf{w}_{Flow }$ to damp the advection dominance.
We choose:
\begin{align*}
\Sta &= c^{1/2} \beta^{1/2} 2 e^t \cos(\pi x)\\
\Adj &= c^{1/2} \beta^{1/2}(e^T-e^t) \cos(\pi x).
\end{align*}
Then, from the gradient equation, we get:
\begin{align*}
\mathbf{w}_{Flow }&= c \beta \frac{2\pi}{\beta}e^t(e^T -e^t)\cos(\pi x) \sin(\pi x)\\
&= c 2\pi e^t(e^T -e^t)\cos(\pi x) \sin(\pi x),
\end{align*}
where it can be noted that $\beta$ is cancelled out.
Again the choice is to set:
\begin{align*}
\nabla \cdot (\rho \mathbf{w}_{Flow}) = \nabla \cdot (\Sta \nabla V_{ext}),
\end{align*}
which implies that
\begin{align*}
\mathbf{w}_{Flow} &= \nabla V_{ext} \\
&= c 2\pi e^t(e^T -e^t)\cos(\pi x) \sin(\pi x).
\end{align*}
Then, integrating this, we find $V_{ext}$:
\begin{align*}
V_{ext} &= \int_\Omega c 2\pi e^t(e^T -e^t)\cos(\pi x) \sin(\pi x) dx\\
&=c e^t(e^T -e^t)\sin^2(\pi x).
\end{align*}

The remaining terms to balance in the forward equation are again:
\begin{align*}
\partial_t \Sta - \nabla^2 \Sta  = {w}_{Force} + f.
\end{align*}
This is:
\begin{align*}
{w}_{Force} + f= c^{1/2} \beta^{1/2}2e^t \cos(\pi x) + c^{1/2} \beta^{1/2} 2\pi^2 \cos (\pi x),
\end{align*}
where ${w}_{Force} + f$ is again one force term.
Then, from the adjoint equation, as before, we can derive $\hat \Sta$:
\begin{align*}
\hat \Sta &= \partial_t \Adj +\Sta   +  \nabla^2 \Adj\\
&= c^{1/2} \beta^{1/2} (1 -\pi^2)e^t \cos(\pi x) + c^{1/2} \beta^{1/2}\pi^2e^T \cos(\pi x).
\end{align*}







\end{document}